RunCheck2.lean
@@ -1,0 +1,8 @@
+import Trident.Common.Symbolic
+import Trident.Target.Semantics
+import Trident.Proofs.Soundness
+import Trident.Proofs.Checker
+import Trident.Proofs.VectorAddEquiv
+
+open Trident
+#eval symCheckVectorAddTutorial parsedVectorAdd 0 1024 1 2048 0
